verifies again with send_across constraints

src/lib/kuiper/Kuiper.SHMem.fst
@@ -3,10 +3,13 @@ module Kuiper.SHMem
 #lang-pulse
 
 open Pulse.Lib.Core
+open Pulse.Lib.Pervasives
 open Pulse.Lib.SendSync
 open Kuiper.Base
 open Kuiper.Array
 open FStar.Tactics.V2
+open Kuiper.ForEvery
+open Kuiper.Common
 module SZ = Kuiper.SizeT
 module T = FStar.Tactics
 
@@ -86,6 +89,40 @@ let rec live_c_shmems #ds (c : c_shmems ds) (#[T.exact (`1.0R)]f:_) : slprop =
     let c : c_shmem d & c_shmems ds = c in (* coerce *)
     live_c_shmem #d (fst c) #f ** live_c_shmems #ds (snd c) #f
 
+ghost
+fn unfold_live_c_shmems_nil (c : c_shmems []) (#[T.exact (`1.0R)]f:_)
+requires live_c_shmems c #f
+ensures emp
+{
+  rewrite (live_c_shmems c #f)
+      as  emp
+}
+
+ghost
+fn fold_live_c_shmems_nil (c : c_shmems []) (#[T.exact (`1.0R)]f:_)
+ensures live_c_shmems c #f
+{
+  rewrite emp as (live_c_shmems c #f);
+}
+
+ghost
+fn unfold_live_c_shmems_cons #d #ds (c : c_shmems (d::ds)) (#[T.exact (`1.0R)]f:_)
+requires live_c_shmems c #f
+ensures live_c_shmem #d (fst c) #f ** live_c_shmems #ds (snd c) #f
+{
+  rewrite (live_c_shmems c #f)
+      as  (live_c_shmem #d (fst c) #f ** live_c_shmems #ds (snd c) #f)
+}
+
+ghost
+fn fold_live_c_shmems_cons #d #ds (c : c_shmems (d::ds)) (#[T.exact (`1.0R)]f:_)
+requires live_c_shmem #d (fst c) #f ** live_c_shmems #ds (snd c) #f
+ensures live_c_shmems c #f
+{
+  rewrite (live_c_shmem #d (fst c) #f ** live_c_shmems #ds (snd c) #f)
+  as (live_c_shmems c #f);
+}
+
 let rec is_send_across_live_c_shmems_ #ds (c:c_shmems ds) #f (pf:squash (c_shmems_inv c))
 : is_send_across block_of (live_c_shmems #ds c #f)
 = let open FStar.Tactics.Typeclasses in
@@ -120,6 +157,131 @@ ensures live_c_shmems c #f
   as (live_c_shmems c #f);
 }
 
-(* 1xn, shared memory *)
+#push-options "--print_implicits"
+let d_ty d : Type0 = let SHArray ty _ = d in ty
+let d_ty_sized d : Kuiper.Sized.sized (d_ty d) = let SHArray _ #s _ = d in s
+let d_len d : SZ.t = let SHArray _ len = d in len
 
+ghost
+fn unfold_live_c_shmem #d (c:c_shmem d) #f
+requires live_c_shmem c #f
+ensures exists* (s:Seq.seq (d_ty d)). gpu_pts_to_array #(d_ty d) #(d_len d) c #f s
+{
+   rewrite each d as (SHArray (d_ty d) #(d_ty_sized d) (d_len d));
+  reduce_with_steps (live_c_shmem #((SHArray (d_ty d) #(d_ty_sized d) (d_len d))) c #f) 
+                    [delta_only [`%live_c_shmem]; iota]
+}
 
+ghost
+fn fold_live_c_shmem #d (c:c_shmem d) #f
+requires exists* (s:Seq.seq (d_ty d)). gpu_pts_to_array #(d_ty d) #(d_len d) c #f s
+ensures live_c_shmem c #f
+{
+  rewrite each d as (SHArray (d_ty d) #(d_ty_sized d) (d_len d));
+  fold (live_c_shmem #((SHArray (d_ty d) #(d_ty_sized d) (d_len d))) c #f);
+  rewrite each ((SHArray (d_ty d) #(d_ty_sized d) (d_len d))) as d;
+}
+
+ghost
+fn gpu_live_c_shmem_share_underspec
+    (#d:_) (c:c_shmem d) (#f:_) (#k:nat { k > 0 })
+requires
+  live_c_shmem c #f
+ensures 
+  forall+ (_ : natlt k). live_c_shmem c #(f /. Real.of_int k)
+{
+  unfold_live_c_shmem c #f;
+  with v. assert (gpu_pts_to_slice #(d_ty d) #(d_len d) c #f 0 (d_len d) v);
+  gpu_slice_share c 0 (d_len d) k #f;
+  forevery_map
+    (fun _ -> gpu_pts_to_slice #(d_ty d) #(d_len d) c #(f /. Real.of_int k) 0 (d_len d) v)
+    (fun _ -> live_c_shmem c #(f /. Real.of_int k))
+    (fun _ -> fold_live_c_shmem #d c #(f /. Real.of_int k));
+}
+
+ghost
+fn rec gpu_live_c_shmems_share_underspec
+    (#ds:_) (c:c_shmems ds) (#f:_) (#k:nat { k > 0 })
+requires
+  live_c_shmems c #f
+ensures 
+  forall+ (_ : natlt k). live_c_shmems c #(f /. Real.of_int k)
+decreases ds
+{
+  match ds {
+    [] -> {
+      unfold_live_c_shmems_nil c #f;
+      forevery_emp_intro (natlt k);
+      forevery_map 
+        (fun _ -> emp)
+        (fun _ -> live_c_shmems c #(f /. Real.of_int k))
+      (fun _ -> fold_live_c_shmems_nil c #(f/. Real.of_int k))
+
+    }
+    d::ds' ->  {
+      unfold_live_c_shmems_cons c #f;
+      gpu_live_c_shmem_share_underspec (fst c) #f #k;
+      gpu_live_c_shmems_share_underspec (snd c) #f #k;
+      forevery_zip
+        (fun _ -> live_c_shmem (fst c) #(f /. Real.of_int k))
+        _;
+      forevery_map
+        (fun _ ->
+          live_c_shmem (fst c) #(f /. Real.of_int k) **
+          live_c_shmems (snd c) #(f /. Real.of_int k))
+        (fun _ -> 
+           live_c_shmems c #(f /. Real.of_int k))
+      (fun _ ->
+        fold_live_c_shmems_cons #d #ds' c  #(f /. Real.of_int k));        
+    }
+  }
+} 
+
+ghost
+fn gpu_live_c_shmem_gather_underspec
+    (#d:_) (c:c_shmem d) (#f:perm) (#k:nat { k > 0 })
+requires
+  forall+ (_ : natlt k). live_c_shmem c #(f /. Real.of_int k)
+ensures
+  live_c_shmem c #f
+{ 
+  forevery_map #(natlt k)
+    (fun _ -> live_c_shmem c #(f /. Real.of_int k))
+    (fun _ -> exists* v. gpu_pts_to_slice #(d_ty d) #(d_len d) c #(f /. Real.of_int k) 0 (d_len d) v)
+    fn _ { unfold_live_c_shmem c #(f /. Real.of_int k)};
+  gpu_slice_gather_underspec c 0 (d_len d) k;
+  fold_live_c_shmem c #f;
+}
+
+ghost
+fn rec gpu_live_c_shmems_gather_underspec
+    (#ds:_) (c:c_shmems ds) (#f:perm) (#k:nat { k > 0 })
+requires
+  forall+ (_ : natlt k). live_c_shmems c #(f /. Real.of_int k)
+ensures
+  live_c_shmems c #f
+decreases ds
+{
+  match ds {
+    [] -> {
+      drop_ (forall+ (_ : natlt k). live_c_shmems #[] c #(f /. Real.of_int k));
+      fold_live_c_shmems_nil (c <: c_shmems []) #f;
+      rewrite each (Nil #shmem_desc) as ds;
+    }
+
+    d::ds' -> {
+      forevery_map #(natlt k)
+        (fun _ -> live_c_shmems #(d::ds') c #(f /. Real.of_int k))
+        (fun _ -> live_c_shmem #d (fst (c<: c_shmem d & c_shmems ds')) #(f /. Real.of_int k) **
+                  live_c_shmems #ds' (snd (c<: c_shmem d & c_shmems ds')) #(f /. Real.of_int k))
+        fn x { 
+          unfold_live_c_shmems_cons #d #ds' c #(f /. Real.of_int k);  
+        };
+      forevery_unzip _ _;
+      gpu_live_c_shmems_gather_underspec #ds' (snd c) #f #k;
+      gpu_live_c_shmem_gather_underspec #d (fst c) #f #k;
+      fold_live_c_shmems_cons #d #ds' c #f;
+      rewrite each (d::ds') as ds;
+    }
+  }
+} 
