src/lib/data/Kuiper.Matrix.Vectorized.fst
@@ -172,7 +172,7 @@ fn __unget_slice_step
       (Seq.init_ghost (k + 1) (fun x -> macc em i (j + x))));
   gpu_slice_split (core gm) #f #(Seq.init_ghost k (fun x -> macc em i (j + x))) #(seq![macc em i (j + k)]) _ (cell_of_pos l i j + k) _;
   strided_row_major_contiguous l i j (j + k);
-  assert pure (j + k < cols);
+  #set-options "--z3refresh --fuel 0 --ifuel 0 --z3rlimit_factor 2" { assert pure (j + k < cols) }  ;
   assert pure (cell_of_pos l i (j + k) == cell_of_pos l i j + k);
   rewrite
     gpu_pts_to_cell (core gm) #f (cell_of_pos l i j + k) (macc em i (j + k))
